CS146 Lecture 19 March 6 2018
#### Recall:
- ```Mio a``` = ```IO a```
- ```miprint``` = ```putStr```
- ```>>>=``` = ```>>=```
- ```>>>``` = ```>>```
- ```inject``` = ```return```

Cleaner Haskell: "do" notation

- ``e1 >> e2`` -> ``do e1 e2 ; e2``
- ``e1 >>= \p->e2`` -> ``do p<-e1 ; e2``

Then
```
interp (Seq s1 s2) st = do st'<- interp s1 st ; interp s2 st'
interp (IPrint ae) st = do puStr(show(aeval s1 st)) ; return st
interp (SPrint s) st = do putStr s ; return st
```

#### Monads
- IO - example of a Monad
- Any data type with >>=, return operators
- monads help to model otherwise impure behaviour purely
- abstract away the "plumbing" that ensures effects are properly sequenced

---

### Proofs for Imperative Programs
Recall: Fib #'s: F0 = 0, F1 = 1, Fn = F(n-1) + F(n-2) (n>1)

Racket:
```
(define (fib n)
  (if (<= n 1) n
      (+ (fib (- n 1)) (fib (- n 2)))))
```
- Proving (fib n) = Fn -> easy induction
- But we know fib is inefficient
- Better: 2 accumulators

```
(defne (fib-h n fn fnm1)
  (cond [(zero? n) fnm1]
        [(= 1 n) fn]
        [else (fib-h (- n 1) (+ fn fnm1) fn)]))

(define (fib n)
  (fib-h n 1 0))
```
- Structurally recursive on n -> linear time in n

To prove (fib n) = Fn -> Prove (fib-h n 1 0) = Fn

But consider the inductive step:
- (fib-h n 1 0) (n>1)
- -> (fib-h (- n 1) 1 1) <- not the same as inductive hypothesis

Need to state and prove a more general hypothesis:
- (fib-h 5 1 0)
- (fib h 4 1 1)
- (fib-h 3 2 1)
- (fib-h 2 3 2)
- (fib-h 1 5 3) = 5

So prove: For all j, For all i > 1,if fjp1 is Fj+1 and fj is Fj then (fib-h i fjp1 fj) = Fi+j
- straightforward induction

#### What would this look like in SIMP?
- set n initially and mutate (no functions)

```
(vars [(n 10) (fj 1) (fjm1 0) (ans 0)]
  (iif (= n 0)
       (set ans fjm1)
       (seq (while (> n 1)
                (set fjm1 fj)
                (set fj (+ fj fjm1))
                (set n (- n 1)))
             (set ans fj)))
  (print ans))
```
- **WRONG** Set ``fjm1 = fj`` then ``fj = fj + fjmi = fj + fj = 2fj``
- Just doubling
- Updated too early

```
(set fj (+ fj fjm1))
(set fjm1 fj)
```
- Still wrong, update fj too early
- use another var

```
(vars [(n 10) (fj 1) (fjm1 0) (t 0) (ans 0)]
  (iif (= n 0)
       (set ans fjm1)
       (seq (while (> n 1)
                   (set t fj)
                   (set fj (+ fj fjm1))
                   (set fjm1 t)
                   (set n (- n 1)))
       (set ans fj)))
  (print ans))
```
- Now this works, but can we prove it?
- Can we prove that for a given n, this program prints Fn?
- Equiv here- prove that the final value of ans is Fn?
- The statement ans=Fn = true or false?
  - depends on the state at the time the sttmt is evaluated

### Hoare Logic
- Prove triples of the form {P} statement {Q} - "Hoare triples"
- P - precondition, logical stmt about the state before statement runs ("Whats true before")
- Q - postcondition, logical stmt about the state after statement runs ("Whats true after")

Interpretation: "If P is true before statement runs then Q is true after after statement runs"

#### Examples/Rules
- To conlude ```{P} (vars [(x1 v1)...(xn vn)] stmt ...) {Q}``` it suffices to show: ```{Q and x1 = 1 and ... and xn = vn} (seq stmt...) {Q}```
- To conclude ```{P} (seq stmt1 stmt2) {Q}``` it suffices to find a stmt R such that ```{P} stmt1 {R}```, ```{R} stmt2 {Q}```
- Finding {R} can be tricky - May need to adjust P and Q to get an R that works
- SO, to conclude ```{P'} stmt {Q'}``` we can prove ```{P} stmt {Q}``` where ```P' => P``` and ```Q => Q'``` (make sure to get the directions right!)
- To conclude ```{P} (set x exp) {Q}```, P and Q hould be almost the same, only the value of x has changed
  - Q can say nothing about the old value of x
  - Whatever Q says about x must be true about exp before the stmt
  - SO, ```{Q[exp/x]} (set x exp) {Q}```
    - ```{Q[exp/x]}``` = Q with exp replacing x
- To conclude: ```{P} (iif B stmt1 stmt2) {Q}``` it suffices to show: ```{P and B} stmt1 {Q}``` and ```{P and not B} stmt2 {Q}```
- ```(while B stmt...)``` - trickiest
  - If the loop doesn't run: ```{P}(while B stmt...){P}```
    - But at the end of the loop, B must be false: ```{P} (while B stmt...) {P and not B}```
  - If the loop repeats: Whatever was true at the end is true at the beginning *and* B is true
    - ```{P and B} (seq s1 ... sn) {P}```
    - P is preserved by the body of the loop- called a loop invariant
    - Finding the right loop invariant can be tricky

Now- prove that the Fib program (simplified) works


```
(vars [(n 10) (fj 1) (fjm1 0) (t 0) (ans 0)]
  ; n=10, fj=F(1), fjm1=F(0), t=0
  ; fj = F(11-n), fjm1=F(10-n) - loop invariant
  (while (not (= n 1))
    (set t fj)
    (set fj (+ fj fjm1))
    (set fjm1 t)
    (set n (- n 1))))
; fj = F(11-n), fjm1 = F(10-n), n=1 - if true at end implies goal
; fj = F(10) -goal
```
- **SO: prove that the loop implies / holds said invariant**
