CS146 Lecture 20 March 7 2018
### Recall:
```
(vars [(n 10) (fj 1) (fjm1 0) (t 0) (ans 0)]
  ; n=10, fj=F(1), fjm1=F(0), t=0
  ; fj = F(11-n), fjm1=F(10-n) - loop invariant
  (while (not (= n 1))
    (set t fj)
    (set fj (+ fj fjm1))
    (set fjm1 t)
    (set n (- n 1))))
; fj = F(11-n), fjm1 = F(10-n), n=1 - if true at end implies goal
; fj = F(10) -goal
```

Just need to prove the loop invariant:
- We work bottom up

```
; fj = F(11-n), fjm1 = F(10-n), not (n = 1)
(seq
; fj + fjm1 = F(12-n), fj = F(11-n) - Not quite the same as the top, but is implied by it
     (set t fj)
; fj + fjm1 = F(12-n), t = F(11-n)
     (set fj (+ fj fjm1))
; replace fjm1 with t: fj = F(12-n), t = F(11-n)     
     (set fjm1 t)
; replace n with n - 1: fj = F(12-n), fjm1 = F(11-n)
     (set n (- n 1)))
; fj = F(11-n), fjm1 = F(10-n)
```
- At the top, we have fj = F(11-n), fjm1 = F(10-n)
- implies fj = F(11-n), fj + fjm1 = F(11-n) + F(10-n) = F(11-n+1) = F(12-n)
